Let expression and big step semantics

expression.v
@@ -2,11 +2,14 @@ Set Warnings "-notation-overridden,-parsing,-deprecated-hint-without-locality".
 From Coq Require Import Strings.String.
 Require Import PeanoNat.
 Require Import nvalue.
+Require Import Bool.
 
 
 Inductive ty : Type :=
   | Ty_Builtin : Type -> ty
   | Ty_Arrow : ty -> ty -> ty.
+
+Check Ty_Builtin nat.
 
 Inductive tm: Type :=
   | tm_var : string -> tm
@@ -19,7 +22,8 @@ Inductive tm: Type :=
   | tm_succ : tm -> tm
   | tm_pred : tm -> tm 
   | tm_mult : tm -> tm -> tm
-  | tm_nvalue (A:Type) : nvalue A -> tm.
+  | tm_nvalue (A:Type) : nvalue A -> tm
+  | tm_val : string -> tm -> tm -> tm.
 
 Declare Custom Entry acnotation.
 
@@ -43,6 +47,12 @@ Notation "'fun' name [ x :  t ]  { y }" :=
 Notation "x y " := (tm_app x y) (in custom acnotation at level 1, left associativity).
 Notation "( x )" := x (in custom acnotation, x at level 99).
 Notation "x" := x (in custom acnotation at level 0, x constr at level 0).
+
+Notation "'val' name = x ; y" := (tm_val name x y) (in custom acnotation at level 90,
+                                                    name at level 99,
+                                                    x custom acnotation at level 99,
+                                                    y custom acnotation at level 99,
+                                                    left associativity).
 
 Notation "S -> T" := (Ty_Arrow S T) (in custom acnotation at level 50, right associativity).
 
@@ -77,7 +87,7 @@ Notation "[ x >> y ] m" := ( device _ x y m)(in custom acnotation at level 30,
                                             x at level 99, 
                                             y at level 99, 
                                             m custom acnotation at level 30).
-(* <{ [5 >> 6] [5 >> 9] [ > 6 ]}> *)
+(* <{ [4 >> 6] [5 >> 9] [ > 6 ]}> *)
 (* <{ [id   value] [id   value] [default] }> *)
 Coercion tm_nvalue: nvalue >-> tm.
 Notation "'NvalueNat'" := (Ty_Builtin (nvalue nat)) (in custom acnotation at level 0).
@@ -105,7 +115,7 @@ Fixpoint subst (x : string) (s : tm) (t : tm) : tm :=
   | tm_var y =>
       if String.eqb x y then s else t
   | <{fun n [y:T] {t1}}> =>
-      if String.eqb x y then t else <{fun n [y:T] {/x:=s/ t1}}>
+      if ((String.eqb x y) || (String.eqb x n)) then t else <{fun n [y:T] {/x:=s/ t1}}>
   | <{t1 t2}> =>
       <{(/x:=s/ t1) (/x:=s/ t2)}>
   | <{true}> =>
@@ -124,10 +134,11 @@ Fixpoint subst (x : string) (s : tm) (t : tm) : tm :=
     <{(/x:=s/ t1) * (/x:=s/ t2)}>
   | tm_nvalue x nv =>
     <{nv}>
+  | <{val n = t1 ; t2}> =>
+    if (String.eqb x n) then t else <{val n = (/x:=s/ t1) ; (/x:=s/ t2)}>
   end
 where "'/' x ':=' s '/' t" := (subst x s t) (in custom acnotation).
 Hint Constructors value : core.
-
 
 Reserved Notation "t '-->' t'" (at level 40).
 Inductive step : tm -> tm -> Prop :=
@@ -151,6 +162,57 @@ Inductive step : tm -> tm -> Prop :=
   | ST_succ: forall (n:nat) (m:nat), m = S (n) -> <{succ n}> --> <{m}>
   | ST_pred: forall (n:nat) (m:nat), m = Nat.pred n -> <{pred n}> --> <{m}>
   | ST_prod: forall (n:nat) (m:nat) (r:nat), r = n * m -> <{n * m}> --> <{r}>
+  | ST_Let1: forall n t1 t1' t2, t1 --> t1' -> 
+            <{val n = t1 ; t2}> --> <{val n = t1' ; t2}>
+  | ST_LetValue: forall n v1 t2, value v1 -> <{val n = v1 ; t2}> --> <{ /n:=v1/t2}>
 where "t '-->' t'" := (step t t').
 
+(*multi-step*)
+Definition relation (X : Type) := X -> X -> Prop.
+Inductive multi {X : Type} (R : relation X) : relation X :=
+  | multi_refl : forall (x : X), multi R x x
+  | multi_single : forall (x y: X), R x y -> multi R x y
+  | multi_step : forall (x y z : X),
+                    R x y ->
+                    multi R y z ->
+                    multi R x z.
+Notation multistep := (multi step).
+Notation "t1 '-->*' t2" := (multistep t1 t2) (at level 40).
+
+
+Reserved Notation "t '==>' t'" (at level 40).
+Inductive bigstep : tm -> tm -> Prop :=
+
+  | ST_Val : forall n t1 t2 w1 w2,
+    <{t1}> ==> <{w1}> ->
+    <{/n := w1/ t2 }> ==> <{w2}> ->
+    <{val n = t1 ; t2}> ==> <{w2}>
+
+  | ST_App : forall v t1 t2' t2 w,
+    value v ->
+    <{t1}> ==> v ->
+    <{t2}> ==> <{t2'}> ->
+    <{v t2'}> ==> <{w}> ->
+    <{t1 t2}> ==> <{w}>
+
+  | ST_Fun : forall n x T2 t1 v w,
+    value v ->
+    <{ /n:=(fun n [x:T2] {t1})/ /x:=v/ t1 }> ==> <{w}> ->
+    <{(fun n [x:T2] {t1}) v}> ==> <{w}>
+
+  | ST_Succ: forall (n:nat) (m:nat), m = S (n) -> <{succ n}> ==> <{m}>
+  | ST_Pred: forall (n:nat) (m:nat), m = Nat.pred n -> <{pred n}> ==> <{m}>
+  | ST_Prod: forall (n:nat) (m:nat) (r:nat), r = n * m -> <{n * m}> ==> <{r}>
+
+  | ST_If_T: forall t1 t2 t3,
+    <{t1}> ==> <{true}> ->
+    <{if0 t1 then t2 else t3}> ==> <{t2}>
+
+  | ST_If_F: forall t1 t2 t3,
+    <{t1}> ==> <{false}> ->
+    <{if0 t1 then t2 else t3}> ==> <{t3}>
+
+  | ST_Refl: forall t1, <{t1}> ==> <{t1}>
+
+where "t '==>' t'" := (bigstep t t').
 
