expression_test.v
@@ -1,0 +1,33 @@
+Require Import expression.
+Require Import String.
+Definition n:string := "n".
+
+Lemma val_test: <{val n = (5*5) ; n * 2}> -->* 50.
+Proof.
+apply multi_step with (y := <{val n = 25 ; n * 2}>).
+apply ST_Let1. apply ST_prod. reflexivity.
+apply multi_step with (y := <{25*2}>).
+apply ST_LetValue. apply v_nat.
+apply multi_single. apply ST_prod. reflexivity.
+Qed.
+
+
+Lemma bigstep_val: <{val n = (5*5) ; n * 2}> ==> 50.
+Proof.
+apply ST_Val with (w1:=25). 
+-apply ST_Prod. reflexivity.
+-simpl. apply ST_Prod. reflexivity.
+Qed.
+
+Definition prod5: string := "prod5".
+Lemma bigstep_fun: <{fun prod5 [x:Nat] {x * 5} 5}> ==> 25.
+Proof.
+apply ST_Fun. simpl.
+- apply v_nat.
+- apply ST_Prod. reflexivity.
+Qed.
+
+
+
+
+
